op-supernode/dafny-models/ChainContainer.dfy
@@ -1,0 +1,30 @@
+include "Types.dfy"
+
+class ChainContainer {
+    function ConfirmedTimestampFor(block : BlockID) : Option<uint64>
+        // No reads clause so it's independent of the current state
+    
+    method PruneDeniedAtOrAfterTimestamp(timestamp : uint64) returns (success : bool)
+        modifies this
+    
+    method RewindEngine(timestamp : uint64) returns (success : bool)
+        modifies this
+
+    method InvalidateBlock(height : uint64, payloadHash : Hash, decisionTimestamp : uint64) returns (rewindTriggered : Option<bool>)
+        modifies this
+
+    method OptimisticAt(ts : uint64) returns (l2AndL1 : OkOrErr<(BlockID, BlockID)>)
+        ensures{:axiom} l2AndL1.Ok? ==>
+            var confirmedTS := ConfirmedTimestampFor(l2AndL1.value.0);
+            confirmedTS != None && confirmedTS.value <= ts
+
+    method FetchReceipts(blockID : BlockID) returns (fetched : Option<(BlockInfo, seq<Receipt>)>)
+        ensures{:axiom} fetched != None ==> fetched.value.0.ID == blockID
+        ensures{:axiom} (fetched != None && ConfirmedTimestampFor(blockID) != None) ==>
+            ConfirmedTimestampFor(blockID).value == fetched.value.0.Time
+
+    method SyncStatus() returns (status : Option<SyncStatus>)
+
+    function BlockTime() : uint64
+        reads this
+}
