op-supernode/dafny-models/LogsDB.dfy
@@ -1,0 +1,154 @@
+include "Types.dfy"
+
+class LogsDB {
+    ghost function View() : seq<BlockRef>
+        reads this
+
+    ghost function LastTimestamp() : uint64
+        reads this
+        requires View() != []
+    {
+        var view := View();
+        view[|view| - 1].Time
+    }
+
+    ghost predicate Invariants()
+        reads this
+    {
+        var view := View();
+
+        (forall i :: 0 < i < |view| ==> view[i - 1].ID.Number == view[i].ID.Number - 1) &&
+        (forall i :: 0 < i < |view| ==> view[i - 1].ID.Hash == view[i].ParentHash) &&
+        (forall i :: 0 < i < |view| ==> view[i - 1].Time <= view[i].Time) // Technically <, except for the first block
+    }
+
+    ghost predicate IsUpperBound(ts : uint64)
+        reads this
+    {
+        forall block :: block in View() ==> block.Time <= ts
+    }
+
+    lemma LastTimestampIsUpperBound()
+        requires Invariants()
+        requires View() != []
+        ensures IsUpperBound(LastTimestamp())
+    {
+        var view := View();
+
+        assert 0 < |view|;
+        assert view[|view| - 1].Time <= LastTimestamp();
+        
+        var i := |view| - 2;
+
+        while 0 <= i
+            invariant forall j :: (i < j < |view| && 0 <= j) ==> view[j].Time <= LastTimestamp()
+        {
+            assert view[i].Time <= view[i + 1].Time;
+
+            i := i - 1;
+        }
+    }
+
+    ghost function Find(number : uint64, list : seq<BlockRef>) : Option<nat>
+        ensures match Find(number, list) {
+            case None =>
+                forall block :: block in list ==> block.ID.Number != number
+            case Some(i) =>
+                i < |list| && list[i].ID.Number == number
+        }
+    {
+        var length := |list|;
+        
+        if length == 0 then
+            None
+        else if list[length - 1].ID.Number == number then
+            Some(length - 1)
+        else
+            Find(number, list[..length - 1])
+    }
+
+    ghost function TimestampForBlock(number : uint64) : Option<uint64>
+        reads this
+    {
+        var view := View();
+        
+        match Find(number, view) {
+            case None => None
+            case Some(index) => Some(view[index].Time)
+        }
+    }
+
+    ghost predicate BlockTimestampIsAtMost(blockNumber : uint64, upperBound : uint64)
+        reads this
+    {
+        TimestampForBlock(blockNumber) == None ||
+        TimestampForBlock(blockNumber).value <= upperBound
+    }
+    
+    function LatestSealedBlock() : Option<BlockID>
+        reads this
+        ensures{:axiom}
+            var view := View();
+            match LatestSealedBlock() {
+                case None =>
+                    view == []
+                case Some(block) =>
+                    0 < |view| && view[|view| - 1].ID == block
+            }
+
+    method Rewind(newHead : BlockID) returns (success : bool)
+        modifies this
+        ensures{:axiom} success ==>
+            var oldView := old(View());
+            var newView := View();
+            var index := Find(newHead.Number, oldView);
+            index != None &&
+            oldView[index.value].ID == newHead &&
+            newView == oldView[..index.value + 1]
+        ensures{:axiom} !success ==> View() == old(View())
+        // Note: The above might not be satisfied by the implementation, meaning that
+        // if Rewind() fails, we can't guarantee the database state hasn't changed
+
+    method Clear() returns (success : bool)
+        modifies this
+        ensures{:axiom} success ==> View() == []
+        ensures{:axiom} !success ==> View() == old(View())
+        // Note: Unsure if we can guarantee the above
+
+    method Contains(query : ContainsQuery) returns (success : bool)
+        ensures{:axiom}
+            var view := View();
+            var index := Find(query.BlockNum, view);
+            assert index != None ==> view[index.value].ID.Number == query.BlockNum;
+            success ==> (index != None && view[index.value].Time == query.Timestamp)
+
+    method FindSealedBlock(number : uint64) returns (seal : Option<BlockSeal>)
+        ensures{:axiom}
+            match seal {
+                case None =>
+                    forall block :: block in View() ==> block.ID.Number != number
+                case Some(block) =>
+                    var view := View();
+                    var index := Find(number, view);
+                    index != None &&
+                    view[index.value].ID.Number == block.Number &&
+                    view[index.value].ID.Hash == block.Hash &&
+                    view[index.value].Time == block.Timestamp &&
+                    block.Number == number
+            }
+
+    method SealBlock(parentHash : Hash, block : BlockID, timestamp : uint64) returns (success : bool)
+        modifies this
+        ensures{:axiom}
+            var oldView := old(View());
+            var newView := View();
+            if !success then
+                newView == oldView // Assume state doesn't change on failure
+            else
+                newView == oldView + [BlockRef(block, parentHash, timestamp)] &&
+                (oldView != [] ==> oldView[|oldView| - 1].ID.Hash == parentHash)
+
+    method AddLog(log : Log, parentBlock : BlockID, logIdx : nat) returns (success : bool)
+        modifies this
+        ensures{:axiom} View() == old(View())
+}
